coq-osiris/theories/program_logic/protocols.v
@@ -1,0 +1,102 @@
+(** *Protocols
+
+    Protocols (following Vilhena and Pottier's [A Separation Logic for Effect
+    Handlers]), describe what effects a computation may perform. *)
+
+From iris.base_logic.lib Require Import iprop.
+
+From osiris Require Export semantics.
+From osiris Require Import util.order.
+
+(* We characterize protocols abstractly, with a carrier type [A], paired with
+   primitive operations [protocol_op]. *)
+
+(* Operations over protocols of carrier [A] *)
+Class protocol_op {A} :=
+  { (* Operation on protocols *)
+    prot_abort : A;
+    prot_sum : A -> A -> A;
+  (* LATER: Support for [f # Ψ] (see Vilhena & Pottier) *)}.
+
+(* The three-place predicate [prot_spec] (analogous to Ψ allows do v {Φ} in
+    Vilhena & Pottier) describes the behavior of a protocol.
+
+   Quoting Vihena & Pottier,
+
+   [prot_spec Ψ v Φ] means that: the "protocol Ψ allows making the request v"
+    and additionally "the protocol Ψ guarantee(s) that every permitted reply
+    satisfies the postcondition Φ."
+
+    Additionally, we require with [prot_spec_ne] that the predicate respects the
+    equivalences for the step-indexed logic of Iris. *)
+Class protocol_spec Σ {A} `{@protocol_op A} :=
+  { prot_spec : A -d> C.eff -d> (syntax.val -d> iProp Σ) -d> iProp Σ ;
+    prot_spec_ne :: forall a e n, Proper ((dist n) ==> (dist n)) (prot_spec a e) }.
+
+Arguments protocol_spec {_ _ _}.
+Arguments prot_spec {_ _ _ _} _ _ _.
+
+(* Protocols, with operations and protocol predicate with carrier type [A] and
+    preorder relation. *)
+Class protocol (Σ : gFunctors) {A} :=
+  { protocol_operations :: @protocol_op A;
+    protocol_specification :: @protocol_spec Σ A _;
+    protocol_preorder :: preorder Σ A }.
+
+Notation "P + Q" := (prot_sum P Q).
+Notation "Ψ 'allows' 'do' v { Φ }" := (prot_spec Ψ v Φ) (at level 40).
+
+(* Axiomatic characterization of protocols. *)
+Section protocol_spec_properties.
+
+  Variable (Σ : gFunctors).
+  Context {A : Type}.
+  Context {Protocol : @protocol Σ A}.
+
+  (* The protocol is monotone over the postcondition and the ordering on protocols. *)
+  Class protocol_monotone :=
+    prot_mono v Ψ1 Ψ2 Φ1 Φ2 :
+      prot_spec Ψ1 v Φ1 ∗ (∀ w, Φ1 w -∗ Φ2 w) ∗ Ψ1 ⊆ Ψ2 ⊢
+        prot_spec Ψ2 v Φ2.
+
+  (* [prot_abort] is logically equivalent to [False]. *)
+  Class protocol_abort :=
+    prot_abort_absurd v Φ :
+      (prot_spec prot_abort v Φ ⊣⊢ ⌜False⌝)%I.
+
+  (* [prot_sum] corresponds to logical or [∨]. *)
+  Class protocol_sum_or :=
+    prot_sum_or v Ψ1 Ψ2 Φ :
+      prot_spec (Ψ1 + Ψ2) v Φ ⊣⊢
+        prot_spec Ψ1 v Φ ∨ prot_spec Ψ2 v Φ.
+
+  (* The set of axiomatic properties that we support on protocols.
+
+     N.B. the [A2; A3; A5] corresponds to the labelling of laws in Vilhena &
+      Pottier. *)
+  Class protocol_properties :=
+  { (* [A2] *)
+    prot_prop_abort :: protocol_abort;
+    (* [A3] *)
+    prot_prop_sum :: protocol_sum_or;
+    (* [A5] *)
+    prot_prop_mono :: protocol_monotone;
+  }.
+
+End protocol_spec_properties.
+
+(* Definition of well-formed protocols, i.e. protocol operations and spec
+   that satisfies certain axiomatic properties. *)
+Class protocol_wf Σ {A} :=
+  { protocol_def :: @protocol Σ A;
+    protocol_wf_properties :: protocol_properties Σ }.
+
+From iris.proofmode Require Import proofmode.
+
+Lemma prot_mono_post {Σ P} `{protocol_wf Σ P}:
+  ∀ Ψ v Φ1 Φ2,
+    ⊢ prot_spec Ψ v Φ1 ∗ (∀ w, Φ1 w -∗ Φ2 w) -∗ prot_spec Ψ v Φ2.
+Proof.
+  iIntros (????) "[HΨ Hmono]".
+  iApply prot_mono; iFrame. iApply refl.
+Qed.
